# own prefixes
@prefix cosn: <https://paul.ti.rw.fau.de/~ju32haqi/supply-networks/abstraction-examples/cosn-ontology#> .
@prefix isn: <https://paul.ti.rw.fau.de/~ju32haqi/supply-networks/abstraction-examples/isn-ontology#> .
@prefix ptsn: <https://paul.ti.rw.fau.de/~ju32haqi/supply-networks/abstraction-examples/ptsn-ontology#> .
@prefix sn: <https://purl.org/supply-network/onto#> .

# other prefixes
@prefix dct: <http://purl.org/dc/terms/> .
@prefix foaf: <http://xmlns.com/foaf/0.1/> .
@prefix owl: <http://www.w3.org/2002/07/owl#> .
@prefix prov: <http://www.w3.org/ns/prov#> .
@prefix qb: <http://purl.org/linked-data/cube#> .
@prefix rdfs: <http://www.w3.org/2000/01/rdf-schema#> .
@prefix schema: <https://schema.org/> .
@prefix vann: <http://purl.org/vocab/vann/> .
@prefix voaf: <http://purl.org/vocommons/voaf#> .
@prefix xsd: <http://www.w3.org/2001/XMLSchema#> .

cosn: a owl:Ontology ;
    rdfs:label "Continent Supply Network Ontology"@en ;
    dct:title "Continent Supply Network Ontology"@en ;
    dct:created "2025-02-06"^^xsd:date ;
    dct:creator <https://danielhenselmann.solidcommunity.net/profile/card#me> ;
    dct:publisher [ foaf:name "Center for Applied Research on Supply Chain Services at Fraunhofer IIS"@en ;
        foaf:homepage <https://www.scs.fraunhofer.de/en.html> ] ;
    dct:license <https://creativecommons.org/licenses/by/4.0/> ;
    voaf:extends qb: , sn: , isn: , ptsn: ;
    rdfs:isDefinedBy cosn: .

<https://danielhenselmann.solidcommunity.net/profile/card#me> foaf:name "Daniel Henselmann" .


# --- classes ---

cosn:Continent a owl:Class ;
    rdfs:subClassOf sn:Entity  ;
    rdfs:label "Continent"@en ;
    rdfs:comment "A geopolictical continent."@en ;
    rdfs:isDefinedBy cosn: .


# --- object properties ---

cosn:export a owl:ObjectProperty , owl:FunctionalProperty , qb:DimensionProperty ;
    rdfs:subPropertyOf sn:from ;
    rdfs:domain sn:SupplyFlow ;
    rdfs:range cosn:Continent ;
    rdfs:label "export"@en ;
    rdfs:comment "Links the exporting continent in a supply flow between two continents."@en ;
    rdfs:isDefinedBy cosn: .

cosn:import a owl:ObjectProperty , owl:FunctionalProperty , qb:DimensionProperty ;
    rdfs:subPropertyOf sn:into ;
    rdfs:domain sn:SupplyFlow ;
    rdfs:range cosn:Continent ;
    rdfs:label "import"@en ;
    rdfs:comment "Links the importing continent in a supply flow between two continents."@en ;
    rdfs:isDefinedBy cosn: .


# --- individuals ---

cosn:ContinentDataStructure a sn:Abstraction ;
    sn:followsDataStructure sn:GenericDataStructure ;
    qb:component [ qb:dimension cosn:export ; qb:componentAttachment sn:SupplyFlow ] ,
            [ qb:dimension cosn:import ; qb:componentAttachment sn:SupplyFlow ] ,
            [ qb:dimension sn:time ] ,
            [ qb:measure sn:quantity] ,
            [ qb:attribute sn:unit] ;
    sn:supplyFlowKey cosn:ContinentSupplyFlowKey ;
    sn:similarAbstractionLevel ptsn:ProductTypeDataStructure , isn:IndustryTypeDataStructure ;
    rdfs:label "Continent Data Structure"@en ;
    rdfs:comment "Defines the abstraction of all continent supply networks through the data structure."@en ;
    rdfs:isDefinedBy cosn: .

cosn:ContinentSupplyFlowKey a sn:SupplyFlowKey ;
    sn:followsSupplyFlowKey sn:GenericSupplyFlowKey ;
    qb:componentProperty cosn:export , cosn:import ;
    rdfs:label "Continent Supply Flow"@en ;
    rdfs:comment "Defines the structure of supply flows in all continent supply networks."@en ;
    rdfs:isDefinedBy cosn: .
    