# own prefix
@prefix cosn: <https://purl.org/supply-network/abstraction/continent/onto#> .
@prefix csn: <https://purl.org/supply-network/abstraction/country/onto#> .
@prefix fssn: <https://purl.org/supply-network/abstraction/federalstate/onto#> .
@prefix isn: <https://purl.org/supply-network/abstraction/industry/onto#> .
@prefix sn: <https://purl.org/supply-network/onto#> .

# other prefixes
@prefix dct: <http://purl.org/dc/terms/> .
@prefix foaf: <http://xmlns.com/foaf/0.1/> .
@prefix owl: <http://www.w3.org/2002/07/owl#> .
@prefix prov: <http://www.w3.org/ns/prov#> .
@prefix qb: <http://purl.org/linked-data/cube#> .
@prefix rdfs: <http://www.w3.org/2000/01/rdf-schema#> .
@prefix schema: <https://schema.org/> .
@prefix vann: <http://purl.org/vocab/vann/> .
@prefix voaf: <http://purl.org/vocommons/voaf#> .
@prefix xsd: <http://www.w3.org/2001/XMLSchema#> .

isn: a owl:Ontology ;
    rdfs:label "Industry Supply Network Ontology"@en ;
    dct:title "Industry Supply Network Ontology"@en ;
    dct:abstract "todo."@en ;
    dct:description "todo."@en ;
    schema:image <https://purl.org/supply-network/abstraction/industry/onto/visualization> ;
    owl:versionInfo "1.0.0" ;
    owl:versionIRI <https://purl.org/supply-network/abstraction/industry/onto/1.0.0> ;
    dct:created "2025-01-31"^^xsd:date ;
    dct:creator <https://danielhenselmann.solidcommunity.net/profile/card#me> ;
    dct:publisher [ foaf:name "Center for Applied Research on Supply Chain Services at Fraunhofer IIS"@en ;
        foaf:homepage <https://www.scs.fraunhofer.de/en.html> ] ;
    dct:license <https://creativecommons.org/licenses/by/4.0/> ;
    schema:creativeWorkStatus "Ontology Release"@en ;
    vann:preferredNamespaceUri <https://purl.org/supply-network/abstraction/industry/onto#> ;
    vann:preferredNamespacePrefix "isn" ;
    voaf:extends qb: , sn: , cosn: , csn: , fssn: ;
    rdfs:isDefinedBy isn: .

<https://danielhenselmann.solidcommunity.net/profile/card#me> foaf:name "Daniel Henselmann" .


# --- classes ---

isn:Industry a owl:Class ;
    rdfs:subClassOf sn:Entity  ;
    rdfs:label "Industry"@en ;
    rdfs:comment "An industry sector."@en ;
    rdfs:isDefinedBy isn: .


# --- object properties ---

isn:demand a owl:ObjectProperty , owl:FunctionalProperty , qb:DimensionProperty ;
    rdfs:subPropertyOf sn:into ;
    rdfs:domain sn:SupplyFlow ;
    rdfs:range isn:Industry ;
    rdfs:label "demand"@en ;
    rdfs:comment "Links the demanding industry in a supply flow between two industries."@en ;
    rdfs:isDefinedBy isn: .

isn:supply a owl:ObjectProperty , owl:FunctionalProperty , qb:DimensionProperty ;
    rdfs:subPropertyOf sn:from ;
    rdfs:domain sn:SupplyFlow ;
    rdfs:range isn:Industry ;
    rdfs:label "supply"@en ;
    rdfs:comment "Links the supplying industry in a supply flow between two industries."@en ;
    rdfs:isDefinedBy isn: .


# --- individuals ---

isn:IndustryContinentDataStructure a sn:Abstraction ;
    sn:followsDataStructure sn:GenericDataStructure ;
    qb:component [ qb:dimension isn:supply ; qb:componentAttachment sn:SupplyFlow ] ,
            [ qb:dimension isn:demand ; qb:componentAttachment sn:SupplyFlow ] ,
            [ qb:dimension cosn:export ; qb:componentAttachment sn:SupplyFlow ] ,
            [ qb:dimension cosn:import ; qb:componentAttachment sn:SupplyFlow ] ,
            [ qb:dimension sn:time ] ,
            [ qb:measure sn:quantity] ,
            [ qb:attribute sn:unit] ;
    sn:supplyLinkKey isn:IndustryContinentSupplyFlowKey ;
    sn:higherAbstractionLevel cosn:ContinentDataStructure , isn:IndustryDataStructure ;
    rdfs:label "[Industry, Continent] Data Structure"@en ;
    rdfs:comment "Defines the abstraction of all [industry, continent] supply networks through the data structure."@en ;
    rdfs:isDefinedBy isn: .

isn:IndustryContinentSupplyFlowkKey a sn:SupplyFlowKey ;
    sn:followsSupplyFlowKey sn:GenericSupplyFlowKey ;
    qb:componentProperty isn:supply , isn:demand , cosn:export , cosn:import ;
    rdfs:label "[Industry, Continent] Supply Flow"@en ;
    rdfs:comment "Defines the structure of supply flows in all [industry, continent] supply networks."@en ;
    rdfs:isDefinedBy isn: .

isn:IndustryCountryDataStructure a sn:Abstraction ;
    sn:followsDataStructure sn:GenericDataStructure ;
    qb:component [ qb:dimension isn:supply ; qb:componentAttachment sn:SupplyFlow ] ,
            [ qb:dimension isn:demand ; qb:componentAttachment sn:SupplyFlow ] ,
            [ qb:dimension csn:export ; qb:componentAttachment sn:SupplyFlow ] ,
            [ qb:dimension csn:import ; qb:componentAttachment sn:SupplyFlow ] ,
            [ qb:dimension sn:time ] ,
            [ qb:measure sn:quantity] ,
            [ qb:attribute sn:unit] ;
    sn:supplyLinkKey isn:IndustryCountrySupplyFlowKey ;
    sn:higherAbstractionLevel csn:CountryDataStructure , cosn:ContinentDataStructure , isn:IndustryDataStructure , isn:IndustryContinentDataStructure ;
    rdfs:label "[Industry, Country] Data Structure"@en ;
    rdfs:comment "Defines the abstraction of all [industry, country] supply networks through the data structure."@en ;
    rdfs:isDefinedBy isn: .

isn:IndustryCountrySupplyFlowkKey a sn:SupplyFlowKey ;
    sn:followsSupplyFlowKey sn:GenericSupplyFlowKey ;
    qb:componentProperty isn:supply , isn:demand , csn:export , csn:import ;
    rdfs:label "[Industry, Country] Supply Flow"@en ;
    rdfs:comment "Defines the structure of supply flows in all [industry, country] supply networks."@en ;
    rdfs:isDefinedBy isn: .

isn:IndustryDataStructure a sn:Abstraction ;
    sn:followsDataStructure sn:GenericDataStructure ;
    qb:component [ qb:dimension isn:supply ; qb:componentAttachment sn:SupplyFlow ] ,
            [ qb:dimension isn:demand ; qb:componentAttachment sn:SupplyFlow ] ,
            [ qb:dimension sn:time ] ,
            [ qb:measure sn:quantity] ,
            [ qb:attribute sn:unit] ;
    sn:supplyLinkKey isn:IndustrySupplyFlowKey ;
    sn:similarAbstractionLevel fssn:FederalStateDataStructure , csn:CountryDataStructure , cosn:ContinentDataStructure ;
    rdfs:label "Industry Data Structure"@en ;
    rdfs:comment "Defines the abstraction of all industry supply networks through the data structure."@en ;
    rdfs:isDefinedBy isn: .

isn:IndustryFederalStateDataStructure a sn:Abstraction ;
    sn:followsDataStructure sn:GenericDataStructure ;
    qb:component [ qb:dimension isn:supply ; qb:componentAttachment sn:SupplyFlow ] ,
            [ qb:dimension isn:demand ; qb:componentAttachment sn:SupplyFlow ] ,
            [ qb:dimension fssn:export ; qb:componentAttachment sn:SupplyFlow ] ,
            [ qb:dimension fssn:import ; qb:componentAttachment sn:SupplyFlow ] ,
            [ qb:dimension sn:time ] ,
            [ qb:measure sn:quantity] ,
            [ qb:attribute sn:unit] ;
    sn:supplyLinkKey isn:IndustryFederalStateSupplyFlowKey ;
    sn:higherAbstractionLevel fssn:FederalStateDataStructure , csn:CountryDataStructure , cosn:ContinentDataStructure , isn:IndustryDataStructure , isn:IndustryCountryDataStructure , isn:IndustryContinentDataStructure ;
    rdfs:label "[Industry, Federal State] Data Structure"@en ;
    rdfs:comment "Defines the abstraction of all [industry, product type] supply networks through the data structure."@en ;
    rdfs:isDefinedBy isn: .

isn:IndustryFederalStateSupplyFlowkKey a sn:SupplyFlowKey ;
    sn:followsSupplyFlowKey sn:GenericSupplyFlowKey ;
    qb:componentProperty isn:supply , isn:demand , fssn:export , fssn:import ;
    rdfs:label "[Industry, Federal State] Supply Flow"@en ;
    rdfs:comment "Defines the structure of supply flows in all [industry, product type] supply networks."@en ;
    rdfs:isDefinedBy isn: .

isn:IndustrySupplyFlowKey a sn:SupplyFlowKey ;
    sn:followsSupplyFlowKey sn:GenericSupplyFlowKey ;
    qb:componentProperty isn:supply , isn:demand ;
    rdfs:label "Industry Supply Flow"@en ;
    rdfs:comment "Defines the structure of supply flows in all industry supply networks."@en ;
    rdfs:isDefinedBy isn: .
    