# own prefix
@prefix rdf: <http://www.w3.org/1999/02/22-rdf-syntax-ns#> .
@prefix sn: <https://purl.org/supply-network/onto#> .

# other prefixes
@prefix dct: <http://purl.org/dc/terms/> .
@prefix foaf: <http://xmlns.com/foaf/0.1/> .
@prefix owl: <http://www.w3.org/2002/07/owl#> .
@prefix qb: <http://purl.org/linked-data/cube#> .
@prefix qudt: <http://qudt.org/schema/qudt/> .
@prefix rdfs: <http://www.w3.org/2000/01/rdf-schema#> .
@prefix schema: <https://schema.org/> .
@prefix skos: <http://www.w3.org/2004/02/skos/core#> .
@prefix time: <http://www.w3.org/2006/time#> .
@prefix vann: <http://purl.org/vocab/vann/> .
@prefix voaf: <http://purl.org/vocommons/voaf#> .
@prefix xsd: <http://www.w3.org/2001/XMLSchema#> .

sn: a owl:Ontology ;
    rdfs:label "Abstraction Independent Supply Network Ontology (AISNO)"@en ;
    dct:title "Abstraction Independent Supply Network Ontology (AISNO)"@en ;
    dct:abstract "todo."@en ;
    dct:description "todo."@en ;
    schema:image <https://purl.org/supply-network/onto/visualization> ;
    owl:versionInfo "1.0.0" ;
    owl:versionIRI <https://purl.org/supply-network/onto/1.0.0> ;
    dct:created "2025-07-22"^^xsd:date ;
    dct:creator <https://danielhenselmann.solidcommunity.net/profile/card#me> ;
    dct:contributor <https://aharth.solidcommunity.net/profile/card#me> ;
    dct:publisher [ foaf:name "Center for Applied Research on Supply Chain Services at Fraunhofer IIS"@en ;
        foaf:homepage <https://www.scs.fraunhofer.de/en.html> ] ;
    dct:license <https://creativecommons.org/licenses/by/4.0/> ;
    schema:creativeWorkStatus "Ontology Release"@en ;
    vann:preferredNamespaceUri <https://purl.org/supply-network/onto#> ;
    vann:preferredNamespacePrefix "sn" ;
    voaf:extends qb: , qudt: , time: , skos: ;
    rdfs:isDefinedBy sn: .

<https://danielhenselmann.solidcommunity.net/profile/card#me> foaf:name "Daniel Henselmann" .
<https://aharth.solidcommunity.net/profile/card#me> foaf:name "Andreas Harth" .


# --- classes ---
    
sn:Entity a owl:Class ;
    rdfs:subClassOf skos:Concept ;
    rdfs:label "Entity"@en ;
    rdfs:comment "Abstract class. An entity that can represent a vertex in a supply network on an abstraction."@en ;
    rdfs:isDefinedBy sn: .

sn:SupplyFlow a owl:Class ;
    rdfs:subClassOf qb:Slice ;
    rdfs:label "Supply Flow"@en ;
    rdfs:comment "A directed supply relation between two entities, typically with a volume."@en ;
    rdfs:isDefinedBy sn: .

time:TemporalEntity rdf:type owl:Class ;
    rdfs:label "Temporal entity"@en ;
    rdfs:comment "A temporal interval or instant."@en ;
    rdfs:isDefinedBy time: .

qudt:Unit a owl:Class ;
    rdfs:label "Unit"@en ;
    rdfs:comment "A unit of measure, or unit, is a particular quantity value that has been chosen as a scale for measuring other quantities the same kind (more generally of equivalent dimension)."@en ;
    rdfs:isDefinedBy qudt: .

sn:Volume a owl:Class ;
    rdfs:subClassOf qb:Observation ;
    rdfs:label "Volume"@en ;
    rdfs:comment "A volume of a supply flow."@en ;
    rdfs:isDefinedBy sn: .


# --- object properties ---

sn:abstractSubstitute a owl:ObjectProperty ;
    rdfs:subPropertyOf skos:broader ;
    rdfs:domain sn:Entity ;
    rdfs:range sn:Entity ;
    rdfs:label "abstract substitute"@en ;
    rdfs:comment "Links an associated entity on another abstraction. This property is abstract, i.e. only abstraction-specific subproperties are used with instance data."@en ;
    rdfs:isDefinedBy sn: .
    
sn:from a owl:ObjectProperty , qb:DimensionProperty ;
    rdfs:domain sn:SupplyFlow ;
    rdfs:range sn:Entity ;
    rdfs:label "from"@en ;
    rdfs:comment "Links the entity that is the origin/source of a directed supply flow between two entities. This property is abstract, i.e. only abstraction-specific subproperties are used with instance data."@en ;
    rdfs:isDefinedBy sn: .

sn:into a owl:ObjectProperty , qb:DimensionProperty ;
    rdfs:domain sn:SupplyFlow ;
    rdfs:range sn:Entity ;
    rdfs:label "into"@en ;
    rdfs:comment "Links the entity that is the target of a directed supply flow between two entities. This property is abstract, i.e. only abstraction-specific subproperties are used with instance data."@en ;
    rdfs:isDefinedBy sn: .

sn:time a owl:ObjectProperty , owl:FunctionalProperty , qb:DimensionProperty ;
    rdfs:domain sn:Volume ;
    rdfs:range time:TemporalEntity ;
    rdfs:label "time"@en ;
    rdfs:comment "Links the time instance or interval of a supply flow's volume."@en ;
    rdfs:isDefinedBy sn: .

sn:unit a owl:ObjectProperty , owl:FunctionalProperty , qb:AttributeProperty ;
    rdfs:domain sn:Volume ;
    rdfs:range qudt:Unit ;
    rdfs:label "unit"@en ;
    rdfs:comment "Links the unit of the observed quantity of a supply flow's volume."@en ;
    rdfs:isDefinedBy sn: .

sn:volume a owl:ObjectProperty , owl:InverseFunctionalProperty ;
    rdfs:subPropertyOf qb:observation ;
    rdfs:domain sn:SupplyFlow ;
    rdfs:range sn:Volume ;
    rdfs:label "volume"@en ;
    rdfs:comment "Links a supply flow's volume."@en ;
    rdfs:isDefinedBy sn: .


# --- datatype properties ---

sn:quantity a owl:DatatypeProperty , owl:FunctionalProperty , qb:MeasureProperty ;
    rdfs:subPropertyOf qudt:quantity ;
    rdfs:domain sn:Volume ;
    rdfs:range xsd:decimal ;
    rdfs:label "quantity"@en ;
    rdfs:comment "Links the observed quantity of a supply flow's volume."@en ;
    rdfs:isDefinedBy sn: .


# --- individuals ---
