# own prefix
@prefix sn: <https://purl.org/supply-network/onto#> .

# other prefixes
@prefix dct: <http://purl.org/dc/terms/> .
@prefix foaf: <http://xmlns.com/foaf/0.1/> .
@prefix owl: <http://www.w3.org/2002/07/owl#> .
@prefix prov: <http://www.w3.org/ns/prov#> .
@prefix qb: <http://purl.org/linked-data/cube#> .
@prefix qudt: <http://qudt.org/schema/qudt/> .
@prefix rdfs: <http://www.w3.org/2000/01/rdf-schema#> .
@prefix schema: <https://schema.org/> .
@prefix skos: <http://www.w3.org/2004/02/skos/core#> .
@prefix time: <http://www.w3.org/2006/time#> .
@prefix vann: <http://purl.org/vocab/vann/> .
@prefix voaf: <http://purl.org/vocommons/voaf#> .
@prefix xsd: <http://www.w3.org/2001/XMLSchema#> .

sn: a owl:Ontology ;
    rdfs:label "Supply Network Ontology"@en ;
    dct:title "Supply Network Ontology"@en ;
    dct:abstract "todo."@en ;
    dct:description "todo."@en ;
    schema:image <https://purl.org/supply-network/onto/visualization> ;
    owl:versionInfo "1.0.0" ;
    owl:versionIRI <https://purl.org/supply-network/onto/1.0.0> ;
    dct:created "2025-01-19"^^xsd:date ;
    dct:creator <https://danielhenselmann.solidcommunity.net/profile/card#me> ;
    dct:publisher [ foaf:name "Center for Applied Research on Supply Chain Services at Fraunhofer IIS"@en ;
        foaf:homepage <https://www.scs.fraunhofer.de/en.html> ] ;
    dct:license <https://creativecommons.org/licenses/by/4.0/> ;
    schema:creativeWorkStatus "Ontology Release"@en ;
    vann:preferredNamespaceUri <https://purl.org/supply-network/onto#> ;
    vann:preferredNamespacePrefix "sn" ;
    voaf:extends qb: , qudt: , time: , skos: , prov: ;
    rdfs:isDefinedBy sn: ;
    rdfs:seeAlso <https://purl.org/supply-network/abstraction/continent/onto#> , <https://purl.org/supply-network/abstraction/country/onto#> , <https://purl.org/supply-network/abstraction/enterprise/onto#> , <https://purl.org/supply-network/abstraction/federalstate/onto#> , <https://purl.org/supply-network/abstraction/industry/onto#> , <https://purl.org/supply-network/abstraction/producttype/onto#> .

<https://danielhenselmann.solidcommunity.net/profile/card#me> foaf:name "Daniel Henselmann" .


# --- classes ---

sn:Abstraction a owl:Class ;
    rdfs:subClassOf qb:DataStructureDefinition , skos:Concept , prov:Entity ;
    rdfs:label "Abstraction"@en ;
    rdfs:comment "A specific abstraction of entities that represent a supply network."@en ;
    rdfs:isDefinedBy sn: .
    
sn:Entity a owl:Class ;
    rdfs:subClassOf skos:Concept ;
    rdfs:label "Entity"@en ;
    rdfs:comment "Abstract class. An entity that can represent a vertex in a supply network on an abstraction."@en ;
    rdfs:isDefinedBy sn: .

sn:SupplyFlow a owl:Class ;
    rdfs:subClassOf qb:Slice ;
    rdfs:label "Supply LiFlownk"@en ;
    rdfs:comment "A directed supply relation between two entities, typically with a volume."@en ;
    rdfs:isDefinedBy sn: .

sn:SupplyFlowKey a owl:Class ;
    rdfs:subClassOf qb:SliceKey , prov:Entity ;
    rdfs:label "Supply Flow Key"@en ;
    rdfs:comment "A fixed subset of dimension properties that are fixed for corresponding supply flows."@en ;
    rdfs:isDefinedBy sn: .

sn:SupplyNetwork a owl:Class ;
    rdfs:subClassOf qb:DataSet , prov:Entity ;
    rdfs:label "Supply Network"@en ;
    rdfs:comment "A representation of a supply network as a network of entities an a specific abstraction."@en ;
    rdfs:isDefinedBy sn: .

sn:Volume a owl:Class ;
    rdfs:subClassOf qb:Observation ;
    rdfs:label "Volume"@en ;
    rdfs:comment "A volume of a supply flow."@en ;
    rdfs:isDefinedBy sn: .


# --- object properties ---

sn:abstractSubstitute a owl:ObjectProperty ;
    rdfs:subPropertyOf skos:broader ;
    rdfs:domain sn:Entity ;
    rdfs:range sn:Entity ;
    rdfs:label "abstract substitute"@en ;
    rdfs:comment "Links an associated entity on another abstraction. This property is abstract, i.e. only abstraction-specific subproperties are used with instance data."@en ;
    rdfs:isDefinedBy sn: .

sn:followsDataStructure a owl:ObjectProperty , qb:FunctionalProperty ;
    rdfs:subPropertyOf prov:specializationOf ;
    rdfs:domain sn:Abstraction ;
    rdfs:range sn:Abstraction ;
    rdfs:label "follows data structure"@en ;
    rdfs:comment "Indicates that an abstraction entity follows the generic structure of a supply network."@en ;
    rdfs:isDefinedBy sn: .

sn:followsSupplyFlowKey a owl:ObjectProperty , qb:FunctionalProperty ;
    rdfs:subPropertyOf prov:specializationOf ;
    rdfs:domain sn:SupplyFlowKey ;
    rdfs:range sn:SupplyFlowKey ;
    rdfs:label "follows supply flow key"@en ;
    rdfs:comment "Indicates that a supply flow key entity follows the generic structure of a supply network."@en ;
    rdfs:isDefinedBy sn: .
    
sn:from a owl:ObjectProperty , qb:DimensionProperty ;
    rdfs:domain sn:SupplyFlow ;
    rdfs:range sn:Entity ;
    rdfs:label "from"@en ;
    rdfs:comment "Links the entity that is the origin/source of a directed supply flow between two entities. This property is abstract, i.e. only abstraction-specific subproperties are used with instance data."@en ;
    rdfs:isDefinedBy sn: .

sn:higherAbstractionLevel a owl:ObjectProperty , owl:TransitiveProperty ;
    rdfs:subPropertyOf skos:broaderTransitive ;
    rdfs:domain sn:Abstraction ;
    rdfs:range sn:Abstraction ;
    rdfs:label "higher abstraction level"@en ;
    rdfs:comment "Links an abstraction on higher level."@en ;
    rdfs:isDefinedBy sn: .

sn:inferredFrom a owl:ObjectProperty , owl:FunctionalProperty ;
    rdfs:subPropertyOf prov:wasDerivedFrom ;
    rdfs:domain sn:SupplyNetwork ;
    rdfs:range sn:SupplyNetwork ;
    rdfs:label "inferred from"@en ;
    rdfs:comment "Links the source supply network on a lower abstraction the supply network was inferred from."@en ;
    rdfs:isDefinedBy sn: .

sn:into a owl:ObjectProperty , qb:DimensionProperty ;
    rdfs:domain sn:SupplyFlow ;
    rdfs:range sn:Entity ;
    rdfs:label "into"@en ;
    rdfs:comment "Links the entity that is the target of a directed supply flow between two entities. This property is abstract, i.e. only abstraction-specific subproperties are used with instance data."@en ;
    rdfs:isDefinedBy sn: .

sn:similarAbstractionLevel a owl:ObjectProperty , owl:SymmetricProperty ;
    rdfs:subPropertyOf skos:related ;
    rdfs:domain sn:Abstraction ;
    rdfs:range sn:Abstraction ;
    rdfs:label "similar abstraction level"@en ;
    rdfs:comment "Links an abstraction on similar level."@en ;
    rdfs:isDefinedBy sn: .

sn:structure a owl:ObjectProperty , owl:FunctionalProperty ;
    rdfs:subPropertyOf qb:structure ;
    rdfs:domain sn:SupplyNetwork ;
    rdfs:range sn:Abstraction ;
    rdfs:label "structure"@en ;
    rdfs:comment "The abstraction of the supply nerwork and all entities in it that also defines the structure of the supply network dataset."@en ;
    rdfs:isDefinedBy sn: .

sn:supplyFlow a owl:ObjectProperty ;
    rdfs:subPropertyOf qb:slice ;
    rdfs:domain sn:SupplyNetwork ;
    rdfs:range sn:SupplyFlow ;
    rdfs:label "supply flow"@en ;
    rdfs:comment "Links all supply flows between entities of the supply network."@en ;
    rdfs:isDefinedBy sn: .

sn:supplyFlowKey a owl:ObjectProperty , owl:FunctionalProperty , owl:InverseFunctionalProperty ;
    rdfs:subPropertyOf qb:sliceKey ;
    rdfs:domain sn:Abstraction ;
    rdfs:range sn:SupplyFlowKey ;
    rdfs:label "supply flow key"@en ;
    rdfs:comment "Links the corresponding supply flow key of the abstraction."@en ;
    rdfs:isDefinedBy sn: .

sn:supplyFlowStructure a owl:ObjectProperty , owl:FunctionalProperty ;
    rdfs:subPropertyOf qb:sliceStructure ;
    rdfs:domain sn:SupplyFlow ;
    rdfs:range sn:SupplyFlowKey ;
    rdfs:label "supply flow structure"@en ;
    rdfs:comment "Links the supply flow's structure/key."@en ;
    rdfs:isDefinedBy sn: .

sn:time a owl:ObjectProperty , owl:FunctionalProperty , qb:DimensionProperty ;
    rdfs:domain sn:Volume ;
    rdfs:range time:TemporalEntity ;
    rdfs:label "time"@en ;
    rdfs:comment "Links the time instance or interval of a supply flow's volume."@en ;
    rdfs:isDefinedBy sn: .

sn:unit a owl:ObjectProperty , owl:FunctionalProperty , qb:AttributeProperty ;
    rdfs:domain sn:Volume ;
    rdfs:range qudt:Unit ;
    rdfs:label "unit"@en ;
    rdfs:comment "Links the unit of the observed quantity of a supply flow's volume."@en ;
    rdfs:isDefinedBy sn: .

sn:volume a owl:ObjectProperty ;
    rdfs:subPropertyOf qb:observation ;
    rdfs:domain sn:SupplyFlow ;
    rdfs:range sn:Volume ;
    rdfs:label "volume"@en ;
    rdfs:comment "Links a supply flow's volume."@en ;
    rdfs:isDefinedBy sn: .


# --- datatype properties ---
    
sn:quantity a owl:DatatypeProperty , owl:FunctionalProperty , qb:MeasureProperty ;
    rdfs:subPropertyOf qudt:quantity ;
    rdfs:domain sn:Volume ;
    rdfs:range xsd:decimal ;
    rdfs:label "quantity"@en ;
    rdfs:comment "Links the observed quantity of a supply flow's volume."@en ;
    rdfs:isDefinedBy sn: .


# --- individuals ---

sn:GenericDataStructure a sn:Abstraction ;
    qb:component [ qb:dimension sn:from ; qb:componentAttachment sn:SupplyFlow ] ,
            [ qb:dimension sn:into ; qb:componentAttachment sn:SupplyFlow ] ,
            [ qb:dimension sn:time ] ,
            [ qb:measure sn:quantity] ,
            [ qb:attribute sn:unit] ;
    sn:supplyFlowKey sn:GenericSupplyFlowKey ;
    rdfs:label "Generic Data Structure"@en ;
    rdfs:comment "This individual is informative and defines the generic abstraction of all supply networks through the data structure."@en ;
    rdfs:isDefinedBy sn: .

sn:GenericSupplyFlowKey a sn:SupplyFlowKey ;
    qb:componentProperty sn:from , sn:into ;
    rdfs:label "Generic Supply Flow"@en ;
    rdfs:comment "This individual is informative and defines the generic structure of supply flows in all supply networks."@en ;
    rdfs:isDefinedBy sn: .
